Table/BuiltinExtensions.lean
@@ -3,7 +3,7 @@ import Table.BuiltinExtensions.Numeric
 import Table.BuiltinExtensions.List.Basic
 import Table.BuiltinExtensions.List.Counts
 import Table.BuiltinExtensions.List.Filtering
-import Table.BuiltinExtensions.List.GroupByKey
+import Table.BuiltinExtensions.List.GroupPairsByKey
 import Table.BuiltinExtensions.List.MergeSort
 import Table.BuiltinExtensions.List.Predicates
 import Table.BuiltinExtensions.List.Sieve
